Small example of bounds-calculation with dependent types
This might properly belong in Experiments rather than TestCase.  It demos the
ability to transform from one kind of constants to another kind, and to plug
bounds calculation functions into [var] to get bounds.  There's not currently
any sort of correctness theorem, and I'm not entirely sure what one would look
like.  Probably something that says that if you map a function over the syntax
tree and then interpret, you could instead have first interpreted and then
applied the function.

I'm hopeful that this will provide a template for integrating this version of
the syntax with rsloan-phoas.

src/Reflection/TestCase.v
@@ -1,9 +1,11 @@
+Require Import Coq.omega.Omega Coq.micromega.Psatz.
 Require Import Crypto.Reflection.Syntax.
 Require Export Crypto.Reflection.Reify.
 Require Import Crypto.Reflection.InputSyntax.
 Require Import Crypto.Reflection.CommonSubexpressionElimination.
 Require Crypto.Reflection.Linearize.
 Require Import Crypto.Reflection.WfReflective.
+Require Import Crypto.Reflection.Conversion.
 
 Import ReifyDebugNotations.
 
@@ -70,14 +72,14 @@ Abort.
 Import Linearize.
 
 Goal True.
-  let x := Reify (fun x y => (let a := 1 in let '(c, d) := (2, 3) in a + x + c + d) + y)%nat in
+  let x := Reify (fun x y => (let a := 1 in let '(c, d) := (2, 3) in a + x - a + c + d) + y)%nat in
   pose (InlineConst (Linearize x)) as e.
   vm_compute in e.
 Abort.
 
-Definition example_expr : Syntax.Expr base_type interp_base_type op (Tbase Tnat).
+Definition example_expr : Syntax.Expr base_type interp_base_type op (Arrow Tnat (Arrow Tnat (Tflat _ tnat))).
 Proof.
-  let x := Reify (let x := 1 in let y := 1 in (let a := 1 in let '(c, d) := (2, 3) in a + x + (x + x) + (x + x) - (x + x) + c + d) + y)%nat in
+  let x := Reify (fun z w => let x := 1 in let y := 1 in (let a := 1 in let '(c, d) := (2, 3) in a + x + (x + x) + (x + x) - (x + x) - a + c + d) + y + z + w)%nat in
   exact x.
 Defined.
 
@@ -143,3 +145,57 @@ Section cse.
 End cse.
 
 Compute CSE (InlineConst (Linearize example_expr)).
+
+Module bounds.
+  Record bounded := { lower : nat ; value : nat ; upper : nat }.
+  Definition map_bounded_f2 (f : nat -> nat -> nat) (swap_on_arg2 : bool) (x y : bounded)
+    := {| lower := f (lower x) (if swap_on_arg2 then upper y else lower y);
+          value := f (value x) (value y);
+          upper := f (upper x) (if swap_on_arg2 then lower y else upper y) |}.
+  Definition bounded_pf :=  { b : bounded | lower b <= value b <= upper b }.
+  Definition add_bounded_pf (x y : bounded_pf) : bounded_pf.
+  Proof.
+    exists (map_bounded_f2 plus false (proj1_sig x) (proj1_sig y)).
+    simpl; abstract (destruct x, y; simpl; omega).
+  Defined.
+  Definition mul_bounded_pf (x y : bounded_pf) : bounded_pf.
+  Proof.
+    exists (map_bounded_f2 mult false (proj1_sig x) (proj1_sig y)).
+    simpl; abstract (destruct x, y; simpl; nia).
+  Defined.
+  Definition sub_bounded_pf (x y : bounded_pf) : bounded_pf.
+  Proof.
+    exists (map_bounded_f2 minus true (proj1_sig x) (proj1_sig y)).
+    simpl; abstract (destruct x, y; simpl; omega).
+  Defined.
+  Definition interp_base_type_bounds (v : base_type) : Type :=
+    match v with
+    | Tnat => { b : bounded | lower b <= value b <= upper b }
+    end.
+  Definition interp_op_bounds src dst (f : op src dst) : interp_flat_type_gen interp_base_type_bounds src -> interp_flat_type_gen interp_base_type_bounds dst
+    := match f with
+       | Add => fun xy => add_bounded_pf (fst xy) (snd xy)
+       | Mul => fun xy => mul_bounded_pf (fst xy) (snd xy)
+       | Sub => fun xy => sub_bounded_pf (fst xy) (snd xy)
+       end%nat.
+  Definition constant_bounded t (x : interp_base_type t) : interp_base_type_bounds t.
+  Proof.
+    destruct t.
+    exists {| lower := x ; value := x ; upper := x |}.
+    simpl; split; reflexivity.
+  Defined.
+  Fixpoint constant_bounds t
+    : interp_flat_type_gen interp_base_type t -> interp_flat_type_gen interp_base_type_bounds t
+    := match t with
+       | Tbase t => constant_bounded t
+       | Prod _ _ => fun x => (constant_bounds _ (fst x), constant_bounds _ (snd x))
+       end.
+
+  Definition example_expr_bounds : Syntax.Expr base_type interp_base_type_bounds op (Arrow Tnat (Arrow Tnat (Tflat _ tnat))) :=
+    Eval vm_compute in
+      (fun var => map base_type op interp_base_type interp_base_type_bounds constant_bounds (fun _ x => x) (fun _ x => x) (example_expr (fun t => var t))).
+
+  Compute (fun x xpf y ypf => proj1_sig (Syntax.Interp interp_op_bounds example_expr_bounds
+                                         (exist _ {| lower := 0 ; value := x ; upper := 10 |} xpf)
+                                         (exist _ {| lower := 100 ; value := y ; upper := 1000 |} ypf))).
+End bounds.
